%========== Useful Equations ==========%

\thispagestyle{fancyplain}

\chapter{Useful Equations}
% stuff taken directly from the appendix of the book used to reduce or change
% expressions when solving recurrences.
...

\section{Telescoping Sums}
\label{appendix:equations|eqn:telescoping}
A sum in which subsequent terms cancel each other, leaving only the first and
the last.
\begin{align}
	S &= \sum_{i=1}^{n-1}(a_{i} - a_{i+1}) \\
	&= (a_1-a_2)+(a_2-a_3) + \dots + (a_{n-2}-a{n-1}) + (a_{n-1}-a_n)
	\nonumber \\
	&= (a_1 - a_n) \nonumber
\end{align}

% \section{Summary}
% \label{ch:definitions|sec:asymptotic-notation|sec:summary}
% TODO: list the definitions in a table

